# Practica 3 / Ejercicio 9  
Probar los siguientes teoremas:  
## I. ((P ⇒ Q) ⇒ Q) ⇒ ((Q ⇒ P) ⇒ P)  
```
                                                                                                (SIGUE ABAJO)
                                                                                                --------------------------------------------------------------------------- ⇒e                    -------------------------------------ax
                                                                                                ((P ⇒ Q) ⇒ Q), (Q ⇒ P), P, ¬Q ⊢ Q                                                                ((P ⇒ Q) ⇒ Q), (Q ⇒ P), P, ¬Q ⊢ ¬Q
                                                                                               ---------------------------------------------------------------------------------------------------------------------------------------------- ¬e
                                                                                                ((P ⇒ Q) ⇒ Q), (Q ⇒ P), P, ¬Q ⊢ ⊥
                                                                                               ------------------------------------------ PBC
                                                                                                ((P ⇒ Q) ⇒ Q), (Q ⇒ P), P ⊢ Q
                                               ----------------------------------------ax      ---------------------------------------- ⇒i
                                               ((P ⇒ Q) ⇒ Q), (Q ⇒ P) ⊢ (P ⇒ Q) ⇒ Q          ((P ⇒ Q) ⇒ Q), (Q ⇒ P) ⊢ (P ⇒ Q) 
--------------------------------ax            ---------------------------------------------------------------------------------------- ⇒e
((P ⇒ Q) ⇒ Q), (Q ⇒ P) ⊢ Q ⇒ P               ((P ⇒ Q) ⇒ Q), (Q ⇒ P) ⊢ Q
-----------------------------------------------------------------------------⇒e
((P ⇒ Q) ⇒ Q), (Q ⇒ P) ⊢ P
--------------------------------------------------------------------------- ⇒i
((P ⇒ Q) ⇒ Q) ⊢ (Q ⇒ P) ⇒ P
----------------------------------------- ⇒i
⊢ ((P ⇒ Q) ⇒ Q) ⇒ ((Q ⇒ P) ⇒ P)
```
```
                                                       ((P ⇒ Q) ⇒ Q), (Q ⇒ P), P, ¬Q ⊢ Q
                                                      ------------------------------------------------------------------------------- ⇒e          -------------------------------------- ax
                                                      ((P ⇒ Q) ⇒ Q), (Q ⇒ P), P, ¬Q ⊢ Q                                                           ((P ⇒ Q) ⇒ Q), (Q ⇒ P), P, ¬Q ⊢ ¬Q
                                                      -------------------------------------------------------------------------------------------------------------------------------------- ¬e
                                                      ((P ⇒ Q) ⇒ Q), (Q ⇒ P), P, ¬Q ⊢ ⊥
                                                     ---------------------------------------- ¬i
                                                      ((P ⇒ Q) ⇒ Q), (Q ⇒ P), P, ¬Q ⊢ ¬P
                                                      ------------------------------------------- ⇒i
                                                      ((P ⇒ Q) ⇒ Q), (Q ⇒ P), P, ¬Q ⊢ ¬Q ⇒ ¬P
----------------------------------------------ax     ------------------------------------------------ CONTRAPOSICION
((P ⇒ Q) ⇒ Q), (Q ⇒ P), P, ¬Q ⊢ (P ⇒ Q) ⇒ Q        ((P ⇒ Q) ⇒ Q), (Q ⇒ P), P, ¬Q ⊢ P ⇒ Q
```  
## II. (P ⇒ Q) ⇒ ((¬P ⇒ Q) ⇒ Q)  
```
asd
```
